txn-data-consistency/EP+_TCCv_Invariants.thy
@@ -332,8 +332,8 @@ lemma kvs_of_s_init:
   "kvs_of_s (state_init) = (\<lambda>k. [\<lparr>v_value = undefined, v_writer = T0, v_readerset = {}\<rparr>])" oops
 
 abbreviation not_committing_ev where
-  "not_committing_ev e \<equiv> \<forall>cl kv_map cts sn u'' clk. e \<noteq> RDone cl kv_map sn u'' clk \<and>
-    e \<noteq> WCommit cl kv_map cts sn u'' clk"   
+  "not_committing_ev e \<equiv> \<forall>cl kv_map cts sn u'' clk mmap. e \<noteq> RDone cl kv_map sn u'' clk \<and>
+    e \<noteq> WCommit cl kv_map cts sn u'' clk mmap"   
 
 lemma kvs_of_s_inv:
   assumes "state_trans s e s'"
@@ -555,15 +555,15 @@ lemma read_done_ctx_closed:
 
 \<comment> \<open>write_commit closedness (canCommit)\<close>
 lemma write_commit_WR_onK:
-  assumes "write_commit cl kv_map commit_t sn u'' clk s s'"
+  assumes "write_commit cl kv_map commit_t sn u'' clk mmap s s'"
   shows "R_onK WR (kvs_of_s s') = R_onK WR (kvs_of_s s)" oops (* not proven *)
 
 lemma write_commit_same_rel:
-  assumes "write_commit cl kv_map commit_t sn u'' clk s s'"
+  assumes "write_commit cl kv_map commit_t sn u'' clk mmap s s'"
   shows "R_CC (kvs_of_s s') = R_CC (kvs_of_s s)" oops
 
 lemma write_commit_ctx_closed:
-  assumes "write_commit cl kv_map commit_t sn u'' clk s s'"
+  assumes "write_commit cl kv_map commit_t sn u'' clk mmap s s'"
     and "closed' (kvs_of_s s) (cl_ctx (cls s cl)) (R_CC (kvs_of_s s))"
     and "closed_general {get_wtxn s cl} ((R_CC (kvs_of_s s))\<inverse>)
           (visTx' (kvs_of_s s) (cl_ctx (cls s cl)) \<union> read_only_Txs (kvs_of_s s))"
@@ -726,30 +726,30 @@ lemma set_cts_order_incl_kvs_tids:
 subsubsection \<open>Write commit guard properties\<close>
 
 lemma write_commit_txn_to_vers_get_wtxn:
-  assumes "write_commit cl kv_map cts sn u'' clk gs gs'" 
+  assumes "write_commit cl kv_map cts sn u'' clk mmap gs gs'" 
   and "kv_map k = Some v" 
   shows "txn_to_vers gs k (get_wtxn gs cl) = new_vers (Tn (Tn_cl sn cl)) v" oops
 
 lemma write_commit_seqn:    \<comment> \<open> NOT USED? \<close>
-  assumes "write_commit cl kv_map cts sn u'' clk gs gs'" 
+  assumes "write_commit cl kv_map cts sn u'' clk mmap gs gs'" 
   shows "sn = cl_sn (cls gs cl)" oops
 
 
 subsubsection \<open>Write commit update properties\<close>
 
 lemma write_commit_txn_to_vers_pres:
-  assumes "write_commit cl kv_map cts sn u'' clk gs gs'"
+  assumes "write_commit cl kv_map cts sn u'' clk mmap gs gs'"
   shows "txn_to_vers gs' k = txn_to_vers gs k" oops
 
 
 lemma write_commit_cts_order_update:
-  assumes "write_commit cl kv_map cts sn u'' clk gs gs'"
+  assumes "write_commit cl kv_map cts sn u'' clk mmap gs gs'"
   shows "cts_order gs' k = 
          (if kv_map k = None then cts_order gs k else cts_order gs k @ [get_wtxn gs cl])" oops
 
 
 lemma write_commit_kvs_of_s:
-  assumes "write_commit cl kv_map commit_t sn u'' clk s s'"
+  assumes "write_commit cl kv_map commit_t sn u'' clk mmap s s'"
   shows "kvs_of_s s' = update_kv (Tn_cl sn cl)
                           (write_only_fp kv_map)
                           (view_of (cts_order s) (cl_ctx (cls s cl)))
@@ -787,7 +787,7 @@ lemma read_commit_views_of_s_other_cl_inv:
   shows "views_of_s s' cl' = views_of_s s cl'" oops (* not proven *)
 
 lemma write_commit_views_of_s_other_cl_inv:
-  assumes "write_commit_s cl kv_map cts sn u clk s s'"
+  assumes "write_commit_s cl kv_map cts sn u clk mmap s s'"
     and "reach tps_s s"
     and "cl' \<noteq> cl"
   shows "views_of_s s' cl' = views_of_s s cl'" oops (* not proven *)
